Phi_Semantics/PhiSem_CF_Break.thy
@@ -37,7 +37,7 @@ hide_fact RES.\<phi>CF_break_res_ax
 subsection \<open>Fiction of Scope Frames\<close>
 
 fiction_space \<phi>CF_break =
-  brk_frame :: \<open>RES.brk_frame.basic_fiction o\<^sub>\<I> \<F>_it\<close>
+  brk_frame :: \<open>RES.brk_frame.basic_fiction ;\<^sub>\<I> \<F>_it\<close>
                (identity_fiction_for_partial_mapping_resource RES.brk_frame) ..
 
 hide_fact FIC.\<phi>CF_break_fic_ax
