Phi_Semantics/PhiSem_Mem_C_Base.thy
@@ -5,12 +5,11 @@ begin
 section \<open>Semantics\<close>
 
 debt_axiomatization
-        MemObj_Size :: \<open>TY \<Rightarrow> nat\<close>
+        MemObj_Size     :: \<open>TY \<Rightarrow> nat\<close>
     and idx_step_offset :: \<open>TY \<Rightarrow> nat \<Rightarrow> nat\<close>
   where memobj_size_step : \<open>valid_idx_step T i \<Longrightarrow> MemObj_Size (idx_step_type i T) \<le> MemObj_Size T\<close>
     and idx_step_offset_size:
-          \<open>valid_idx_step T i
-                \<Longrightarrow> idx_step_offset T i + MemObj_Size (idx_step_type i T) \<le> MemObj_Size T\<close>
+          \<open>valid_idx_step T i \<Longrightarrow> idx_step_offset T i + MemObj_Size (idx_step_type i T) \<le> MemObj_Size T\<close>
     and idx_step_offset_disj:
           \<open>valid_idx_step T i \<Longrightarrow> valid_idx_step T j \<Longrightarrow>
                 idx_step_offset T i \<le> idx_step_offset T j \<Longrightarrow>
@@ -32,9 +31,9 @@ lemma fold_tail:
 lemma index_offset_upper_bound:
   \<open>valid_index T (base@idx) \<Longrightarrow>
    index_offset T (base@idx) + MemObj_Size (index_type (base@idx) T) \<le> index_offset T base + MemObj_Size (index_type base T)\<close>
-  apply (induct idx arbitrary: base rule: rev_induct;
-         simp del: append_assoc add: append_assoc[symmetric] fold_tail)
-  using idx_step_offset_size by fastforce
+  by (induct idx arbitrary: base rule: rev_induct;
+      simp del: append_assoc add: append_assoc[symmetric] fold_tail;
+      insert idx_step_offset_size, fastforce)
 
 lemmas index_offset_upper_bound_0 = index_offset_upper_bound[where base = "[]", simplified]
 
@@ -55,19 +54,22 @@ lemma index_offset_bound_strict:
 
 section \<open>Fiction\<close>
 
-debt_axiomatization Mapof_Val :: \<open>VAL \<Rightarrow> nat list \<rightharpoonup> VAL\<close>
-  where Mapof_Val_inj: \<open>Va \<in> Well_Type T \<Longrightarrow> Vb \<in> Well_Type T \<Longrightarrow> Mapof_Val Va = Mapof_Val Vb \<Longrightarrow> Va = Vb\<close>
-  and   Mapof_Val_same_dom: \<open>Va \<in> Well_Type T \<Longrightarrow> Vb \<in> Well_Type T \<Longrightarrow> dom (Mapof_Val Va) = dom (Mapof_Val Vb)\<close>
-  and   Mapof_not_1[simp]: \<open>Mapof_Val V \<noteq> 1\<close>
-  and   Mapof_Val_pull_step: \<open>valid_idx_step T i \<Longrightarrow> V \<in> Well_Type T
-                          \<Longrightarrow> pull_map [i] (Mapof_Val V) = Mapof_Val (idx_step_value i V)\<close>
-  and   Mapof_Val_mod_step: \<open>valid_idx_step T i \<Longrightarrow> v \<in> Well_Type T
-                         \<Longrightarrow> Mapof_Val (idx_step_mod_value i f v) = Mapof_Val v ++ push_map [i] (Mapof_Val (f (idx_step_value i v)))\<close>
+debt_axiomatization Map_of_Val :: \<open>VAL \<Rightarrow> nat list \<rightharpoonup> VAL\<close>
+  where Map_of_Val_inj: \<open>Va \<in> Well_Type T \<Longrightarrow> Vb \<in> Well_Type T \<Longrightarrow> Map_of_Val Va = Map_of_Val Vb \<Longrightarrow> Va = Vb\<close>
+  and   Map_of_Val_same_dom: \<open>Va \<in> Well_Type T \<Longrightarrow> Vb \<in> Well_Type T \<Longrightarrow> dom (Map_of_Val Va) = dom (Map_of_Val Vb)\<close>
+  and   Mapof_not_1[simp]: \<open>Map_of_Val V \<noteq> 1\<close>
+  and   Map_of_Val_pull_step: \<open>valid_idx_step T i \<Longrightarrow> V \<in> Well_Type T
+                          \<Longrightarrow> pull_map [i] (Map_of_Val V) = Map_of_Val (idx_step_value i V)\<close>
+  and   Map_of_Val_mod_step: \<open>valid_idx_step T i \<Longrightarrow> v \<in> Well_Type T
+                         \<Longrightarrow> Map_of_Val (idx_step_mod_value i f v) = Map_of_Val v ++ push_map [i] (Map_of_Val (f (idx_step_value i v)))\<close>
 
-lemma Mapof_Val_pull:
-  \<open>valid_index T idx \<Longrightarrow> V \<in> Well_Type T \<Longrightarrow> pull_map idx (Mapof_Val V) = Mapof_Val (index_value idx V)\<close>
+definition Map_of_Val' :: \<open>VAL nosep \<Rightarrow> nat list \<rightharpoonup> VAL nosep\<close>
+  where \<open>Map_of_Val' V = (map_option nosep o Map_of_Val (nosep.dest V))\<close>
+
+lemma Map_of_Val_pull:
+  \<open>valid_index T idx \<Longrightarrow> V \<in> Well_Type T \<Longrightarrow> pull_map idx (Map_of_Val V) = Map_of_Val (index_value idx V)\<close>
   apply (induct idx arbitrary: V T; simp)
-  using Mapof_Val_pull_step
+  using Map_of_Val_pull_step
   by (metis idx_step_value_welltyp pull_map_cons)
 
 lemma total_Mapof_disjoint:
@@ -81,42 +83,42 @@ lemma map_add_subsumed_dom:
   unfolding map_add_def dom_def subset_eq fun_eq_iff apply simp
   by (metis option.case_eq_if option.collapse option.simps(3))
 
-lemma Mapof_Val_mod:
+lemma Map_of_Val_mod:
   \<open> valid_index T idx
 \<Longrightarrow> v \<in> Well_Type T
 \<Longrightarrow> u \<in> Well_Type (index_type idx T)
-\<Longrightarrow> Mapof_Val (index_mod_value idx (\<lambda>_. u) v) = Mapof_Val v ++ push_map idx (Mapof_Val u)\<close>
+\<Longrightarrow> Map_of_Val (index_mod_value idx (\<lambda>_. u) v) = Map_of_Val v ++ push_map idx (Map_of_Val u)\<close>
   apply (induct idx arbitrary: u v T; simp)
-  using Mapof_Val_same_dom map_add_subsumed_dom apply (metis order_refl)
-  by clarify (simp add: idx_step_value_welltyp Mapof_Val_mod_step  push_map_distrib_map_add
-                        Mapof_Val_pull_step[symmetric] push_pull_map map_add_subsumed2
+  using Map_of_Val_same_dom map_add_subsumed_dom apply (metis order_refl)
+  by clarify (simp add: idx_step_value_welltyp Map_of_Val_mod_step  push_map_distrib_map_add
+                        Map_of_Val_pull_step[symmetric] push_pull_map map_add_subsumed2
                         push_map_push_map)
 
-lemma Mapof_Val_modify_fiction:
+lemma Map_of_Val_modify_fiction:
    \<open>valid_index T idx
 \<Longrightarrow> v \<in> Well_Type T
 \<Longrightarrow> u \<in> Well_Type (index_type idx T)
 \<Longrightarrow> u'\<in> Well_Type (index_type idx T)
-\<Longrightarrow> g ## (push_map idx (to_share \<circ> Mapof_Val u))
-\<Longrightarrow> to_share \<circ> (Mapof_Val v) = g * (push_map idx (to_share \<circ> Mapof_Val u))
-\<Longrightarrow> to_share \<circ> (Mapof_Val (index_mod_value idx (\<lambda>_. u') v)) = g * (push_map idx (to_share \<circ> Mapof_Val u'))\<close>
-  apply (simp add: Mapof_Val_mod to_share_funcomp_map_add push_map_to_share
+\<Longrightarrow> g ## (push_map idx (to_share \<circ> Map_of_Val u))
+\<Longrightarrow> to_share \<circ> (Map_of_Val v) = g * (push_map idx (to_share \<circ> Map_of_Val u))
+\<Longrightarrow> to_share \<circ> (Map_of_Val (index_mod_value idx (\<lambda>_. u') v)) = g * (push_map idx (to_share \<circ> Map_of_Val u'))\<close>
+  apply (simp add: Map_of_Val_mod to_share_funcomp_map_add push_map_to_share
       times_fun_map_add_right total_Mapof_disjoint[simplified push_map_to_share]
-      Mapof_Val_same_dom push_map_dom_eq)
+      Map_of_Val_same_dom push_map_dom_eq)
   subgoal premises prems proof -
-    have \<open>dom g \<inter> dom (to_share \<circ> push_map idx (Mapof_Val u)) = {}\<close>
+    have \<open>dom g \<inter> dom (to_share \<circ> push_map idx (Map_of_Val u)) = {}\<close>
       using prems to_share_total_disjoint by blast
     moreover have t1:
-      \<open>dom (to_share \<circ> push_map idx (Mapof_Val u)) = dom (to_share \<circ> push_map idx (Mapof_Val u'))\<close>
-      using prems by (metis Mapof_Val_same_dom dom_map_option_comp push_map_dom_eq)
-    ultimately have \<open>dom g \<inter> dom (to_share \<circ> push_map idx (Mapof_Val u')) = {}\<close> by metis
+      \<open>dom (to_share \<circ> push_map idx (Map_of_Val u)) = dom (to_share \<circ> push_map idx (Map_of_Val u'))\<close>
+      using prems by (metis Map_of_Val_same_dom dom_map_option_comp push_map_dom_eq)
+    ultimately have \<open>dom g \<inter> dom (to_share \<circ> push_map idx (Map_of_Val u')) = {}\<close> by metis
     note [simp] = times_fun_map_add_right[OF this]
     show ?thesis by simp (metis t1 map_add_subsumed_dom order_eq_refl)
   qed
   done
 (* lemma pull_map_share_Mapof_not_eq_1[simp]:
-  \<open>valid_index (Typeof v) idx \<Longrightarrow> pull_map idx (share n (to_share \<circ> Mapof_Val v)) = 1 \<longleftrightarrow> n = 0\<close>
-  by (cases \<open>n = 0\<close>; simp add: pull_map_share pull_map_to_share Mapof_Val_pull)
+  \<open>valid_index (Typeof v) idx \<Longrightarrow> pull_map idx (share n (to_share \<circ> Map_of_Val v)) = 1 \<longleftrightarrow> n = 0\<close>
+  by (cases \<open>n = 0\<close>; simp add: pull_map_share pull_map_to_share Map_of_Val_pull)
 *)
 
 
@@ -124,47 +126,53 @@ lemma map_add_restrict_itself [simp]: \<open>(f ++ g) |` dom g = g\<close>
   unfolding fun_eq_iff restrict_map_def map_add_def
   by (simp add: domIff option.case_eq_if)
 
-lemma Mapof_Val_inj_plus:
-  \<open>Va \<in> Well_Type T \<Longrightarrow> Vb \<in> Well_Type T \<Longrightarrow> f ++ Mapof_Val Va = f ++ Mapof_Val Vb \<Longrightarrow> Va = Vb\<close>
-proof (rule Mapof_Val_inj, assumption)
+lemma Map_of_Val_inj_plus:
+  \<open>Va \<in> Well_Type T \<Longrightarrow> Vb \<in> Well_Type T \<Longrightarrow> f ++ Map_of_Val Va = f ++ Map_of_Val Vb \<Longrightarrow> Va = Vb\<close>
+proof (rule Map_of_Val_inj, assumption)
   assume tyA: \<open>Va \<in> Well_Type T\<close>
      and tyB: \<open>Vb \<in> Well_Type T\<close>
-     and feq: \<open>f ++ Mapof_Val Va = f ++ Mapof_Val Vb\<close>
-  then have \<open>(f ++ Mapof_Val Va) |` dom (Mapof_Val Va) = (f ++ Mapof_Val Vb) |` dom (Mapof_Val Vb)\<close>
-    using Mapof_Val_same_dom by metis 
+     and feq: \<open>f ++ Map_of_Val Va = f ++ Map_of_Val Vb\<close>
+  then have \<open>(f ++ Map_of_Val Va) |` dom (Map_of_Val Va) = (f ++ Map_of_Val Vb) |` dom (Map_of_Val Vb)\<close>
+    using Map_of_Val_same_dom by metis 
   note this [simplified]
-  then show \<open>Mapof_Val Va = Mapof_Val Vb\<close> .
+  then show \<open>Map_of_Val Va = Map_of_Val Vb\<close> .
 qed
 
-definition \<open>Valof_Map TY M = (@V. (\<exists>f. f ++ Mapof_Val V = M) \<and> V \<in> Well_Type TY)\<close>
+definition \<open>Val_of_Map TY M = (@V. (\<exists>f. f ++ Map_of_Val V = M) \<and> V \<in> Well_Type TY)\<close>
 
-lemma Valof_Map_append[simp]:
-  \<open>v \<in> Well_Type T \<Longrightarrow> Valof_Map T (f ++ Mapof_Val v) = v\<close>
-  unfolding Valof_Map_def
-  using someI[where P=\<open>\<lambda>V. (\<exists>fa. fa ++ Mapof_Val V = f ++ Mapof_Val v) \<and> V \<in> Well_Type T\<close> and x=v, simplified]
-        Mapof_Val_inj_plus
-  by (metis (no_types, lifting) Mapof_Val_same_dom map_add_restrict_itself) 
+lemma Val_of_Map_append[simp]:
+  \<open>v \<in> Well_Type T \<Longrightarrow> Val_of_Map T (f ++ Map_of_Val v) = v\<close>
+  unfolding Val_of_Map_def
+  using someI[where P=\<open>\<lambda>V. (\<exists>fa. fa ++ Map_of_Val V = f ++ Map_of_Val v) \<and> V \<in> Well_Type T\<close> and x=v, simplified]
+        Map_of_Val_inj_plus
+  by (metis (no_types, lifting) Map_of_Val_same_dom map_add_restrict_itself) 
 
-lemmas Valof_Map[simp] = Valof_Map_append[where f = \<open>Map.empty\<close>, simplified]
+lemmas Val_of_Map[simp] = Val_of_Map_append[where f = \<open>Map.empty\<close>, simplified]
+
+
+term \<open>Map_of_Val\<close>
+
+interpretation Val_of_Map: cancl_perm_ins_homo \<open>Map_of_Val\<close>
+
 
 
 lemma
   \<open> perm_ins_homo' f
-\<Longrightarrow> perm_ins_homo' (\<lambda>v. f o Mapof_Val v)\<close>
+\<Longrightarrow> perm_ins_homo' (\<lambda>v. f o Map_of_Val v)\<close>
 
-  term \<open>(\<lambda>v. f o Mapof_Val v)\<close>
-  term Mapof_Val
-  term \<open>((o) to_share) o Mapof_Val\<close>
+  term \<open>(\<lambda>v. f o Map_of_Val v)\<close>
+  term Map_of_Val
+  term \<open>((o) to_share) o Map_of_Val\<close>
 
 
 
 
 
 definition \<open>fic_val_to_share_map TY =
-      Interp (\<lambda>m. if m = 1 then {None} else {Some v |v. v \<in> Well_Type TY \<and> to_share o Mapof_Val v = m})\<close>
+      Interp (\<lambda>m. if m = 1 then {None} else {Some v |v. v \<in> Well_Type TY \<and> to_share o Map_of_Val v = m})\<close>
 
 lemma fic_val_to_share_map[simp]:
-  \<open>\<I> (fic_val_to_share_map TY) = (\<lambda>m. if m = 1 then {None} else {Some v |v. v \<in> Well_Type TY \<and> to_share o Mapof_Val v = m})\<close>
+  \<open>\<I> (fic_val_to_share_map TY) = (\<lambda>m. if m = 1 then {None} else {Some v |v. v \<in> Well_Type TY \<and> to_share o Map_of_Val v = m})\<close>
   unfolding fic_val_to_share_map_def by (rule Interp_inverse) (simp add: Interpretation_def one_set_def)
 
 
