Phi_Semantics/PhiSem_Variable.thy
@@ -43,7 +43,7 @@ hide_fact RES.\<phi>var_res_ax RES.\<phi>var_res_axioms RES.\<phi>var_res_fields
 subsubsection \<open>Fiction\<close>
 
 fiction_space \<phi>var =
-  Var :: \<open>RES.Var.basic_fiction o\<^sub>\<I> \<F>_pointwise \<F>_it\<close> (pointwise_fiction_for_partial_mapping_resource RES.Var) ..
+  Var :: \<open>RES.Var.basic_fiction ;\<^sub>\<I> \<F>_pointwise \<F>_it\<close> (pointwise_fiction_for_partial_mapping_resource RES.Var) ..
 
 hide_fact FIC.\<phi>var_fic_ax FIC.\<phi>var_fic_axioms
 
